@prefix : <http://www.example.org/ontology/hospital#> .
@prefix owl: <http://www.w3.org/2002/07/owl#> .
@prefix rdf: <http://www.w3.org/1999/02/22-rdf-syntax-ns#> .
@prefix xml: <http://www.w3.org/XML/1998/namespace> .
@prefix xsd: <http://www.w3.org/2001/XMLSchema#> .
@prefix rdfs: <http://www.w3.org/2000/01/rdf-schema#> .
@prefix ce: <http://www.ontologydesignpatterns.org/cp/owl/collectionentity.owl#> .

:Article a owl:Class ;
         rdfs:label "Article" ;
         rdfs:comment "A written composition on a particular subject, usually forming an independent part of a book or collection" .

:Book a owl:Class ;
      rdfs:subClassOf ce:Collection ;
      rdfs:label "Book" ;
      rdfs:comment "A collection of pages bound together, containing written information or literature" .

:CD a owl:Class ;
     rdfs:subClassOf ce:Collection ;
     rdfs:label "CD" ;
     rdfs:comment "An optical disc used to store digital data, which can include text articles" .

:hasArticle a owl:ObjectProperty ;
            rdfs:domain [ owl:unionOf (:Book :CD) ] ;
            rdfs:range :Article ;
            rdfs:label "has article" ;
            rdfs:comment "A property indicating the articles contained within a book or CD" .

ce:hasMember a owl:ObjectProperty ;
             rdfs:subPropertyOf :hasArticle ;
             rdfs:domain ce:Collection ;
             rdfs:range owl:Thing ;
             rdfs:label "has member" ;
             rdfs:comment "A relation between collections and entities, indicating membership of an entity in a collection" .

:composedOf a owl:ObjectProperty ;
             owl:inverseOf ce:hasMember ;
             rdfs:domain owl:Thing ;
             rdfs:range ce:Collection ;
             rdfs:label "is composed of" ;
             rdfs:comment "A property indicating the collection to which an entity belongs" .

### Individuals

:Article_NursePracticesInCancerPatientCare a :Article ;
                                             rdfs:label "A 5 year-program for improving cancer care � experiences and future directions" .

:Book_NursePracticesInCancerPatientCare a :Book ;
                                          rdfs:label "Nurse practices in cancer patient care � longitudinal studies at Italian hospitals" ;
                                          ce:hasMember :Article_NursePracticesInCancerPatientCare .

### Restrictions

:Book rdfs:subClassOf [ a owl:Restriction ;
                        owl:onProperty :hasArticle ;
                        owl:someValuesFrom :Article ] .

:CD rdfs:subClassOf [ a owl:Restriction ;
                      owl:onProperty :hasArticle ;
                      owl:someValuesFrom :Article ] .
